kuiops/common/supergemm/output/Kuiops.SuperGEMM.Mm.Output.fsti
@@ -26,6 +26,9 @@ open Kuiper.Kernel.GEMM.Tiled.Common.Vec { block_tile, warp_tile }
 open Kuiper.Kernel.GEMM.TensorCore2D.To.KernelDesc { output_fragment, output_lane_live,
                                                      live_lane_cells }
 
+module SZ = Kuiper.SizeT
+module T = Kuiper.Tensor
+
 inline_for_extraction noextract
 let output_fragment'
   (#et : Type0) {| scalar et |}
@@ -58,3 +61,44 @@ let output_lane_live'
     live_lane_cells
       (output_fragment' gD bm bn tm tn wm wn bid (tid / warp_size) mi nj)
       (tid % warp_size)
+
+(* ---- layout-generic live split of the output tile among warp lanes ----
+   The generalisation of upstream
+   [Kuiper.Kernel.GEMM.TensorCore2D.To.KernelDesc.split_output_to_lanes] to an
+   arbitrary [lD : layout2 m n]. *)
+ghost
+fn split_output_to_lanes'
+  (#et : Type0) {| scalar et, has_vec_cpy et |}
+  (#m #n : szp)
+  (#lD : layout2 (SZ.v m) (SZ.v n)) {| T.ctlayout lD |}
+  (gD : array2 et lD)
+  (bm bn tm tn wm wn : szp)
+  (#_ : squash (bm /?+ m /\ bn /?+ n /\
+                wm * tm /?+ bm /\ wn * tn /?+ bn))
+  (nblk : szp{SZ.v nblk == SZ.v m / SZ.v bm * (SZ.v n / SZ.v bn)})
+  (nthr : szp{SZ.v nthr == SZ.v bm / (SZ.v wm * SZ.v tm) * (SZ.v bn / (SZ.v wn * SZ.v tn)) * warp_size})
+  ()
+  requires live gD
+  ensures
+    forall+ (bid : natlt nblk) (tid : natlt nthr).
+      output_lane_live' gD bm bn tm tn wm wn bid tid
+
+(* ---- layout-generic live inverse of [split_output_to_lanes'] ---- *)
+ghost
+fn gather_output_live'
+  (#et : Type0) {| scalar et, has_vec_cpy et |}
+  (#m #n : szp)
+  (#lD : layout2 (SZ.v m) (SZ.v n)) {| T.ctlayout lD |}
+  (gD : array2 et lD)
+  (bm bn tm tn wm wn : szp)
+  (#_ : squash (bm /?+ m /\ bn /?+ n /\
+                wm * tm /?+ bm /\ wn * tn /?+ bn))
+  (#_ : squash (tm /?+ (wm * tm) /\ tn /?+ (wn * tn)))
+  (#_ : squash (SZ.fits (m * n)))
+  (nblk : szp{SZ.v nblk == SZ.v m / SZ.v bm * (SZ.v n / SZ.v bn)})
+  (nthr : szp{SZ.v nthr == SZ.v bm / (SZ.v wm * SZ.v tm) * (SZ.v bn / (SZ.v wn * SZ.v tn)) * warp_size})
+  ()
+  requires
+    forall+ (bid : natlt nblk) (tid : natlt nthr).
+      output_lane_live' gD bm bn tm tn wm wn bid tid
+  ensures exists* (eD : chest2 et (SZ.v m) (SZ.v n)). gD |-> eD
